
\begin{align}
 &\divergence \nabla v = 0, \\
 &\divergence \gamma \nabla u = 0
\end{align}
\begin{align}
  &\divergence \gamma \nabla w + \divergence (\gamma - 1)\nabla v = 0\textup{ in }\Omega \\
  &\partial_\nu w = 0 \textup{ on }\partial \Omega
\end{align}

The weak formulation is
\begin{equation}
 \int_\Omega \gamma \nabla w\nabla \phi = - \int_D (k-1)\nabla v\nabla \phi 
 \quad \forall\phi \in H^1(\Omega)
\end{equation}

We can rewrite the problem for $w$ as 
\begin{align}
 &\Delta w = 0\textup{ in } \Omega\backslash\overline{D} \textup{ and in }D \\
 & w^+ = w^- \textup{ on }\partial D\\
 & \partial_\nu w^+ = k \partial_\nu w^- + (k-1)\partial_\nu v^- = k\partial_\nu u^- - \partial_\nu v^- \textup{ on }\partial D \\
 & \partial_\nu w = 0 \textup{ on }\partial \Omega
\end{align}

